user 3, session 3788, part 19

diffs-annotated-with-times/3/user-3-session-3788.v
@@ -32,9 +32,35 @@ Redirect "/var/folders/5x/1mdbpbjd7012l971fq0zkj2w0000gn/T/coqoPhort"
 SearchPattern _.
 Remove Search Blacklist "Raw" "Proofs".
 Unset Search Output Name Only.
-Definition change_marker `{m : ProcMarker p} {T'} 
+Definition change_marker `{m : @ProcMarker T p} {T'} 
   (p' : proc T') : ProcMarker p' := AProc p'.
+Redirect "/var/folders/5x/1mdbpbjd7012l971fq0zkj2w0000gn/T/coqfBlXZI"
+Print Ltac Signatures.
+Timeout 1 Print Grammar tactic.
+Add Search Blacklist "Raw" "Proofs".
+Set Search Output Name Only.
+Redirect "/var/folders/5x/1mdbpbjd7012l971fq0zkj2w0000gn/T/coq4luqFX"
+SearchPattern _.
+Remove Search Blacklist "Raw" "Proofs".
+Unset Search Output Name Only.
+Theorem swapXY_ok :
+  proc_spec
+    (fun (_ : unit) state =>
+     {|
+     pre := True;
+     post := fun r state' =>
+             state' = mkState (StateY state) (StateX state) (StateZ state);
+     recovered := fun _ state' => True |}) swapXY vars.recover vars.abstr.
+Proof.
+(match goal with
+ | |- proc_spec _ ?p _ _ => pose proof (AProc p) as Hbefore
+ end).
+(unfold swapXY).
+monad_simpl.
+(match goal with
+ | |- proc_spec _ ?p _ _ => apply (change_marker p) in Hbefore
+ end).
 (* Auto-generated comment: Failed. *)
 
-(* Auto-generated comment: At 2019-08-29 08:53:58.520000.*)
+(* Auto-generated comment: At 2019-08-29 08:54:00.550000.*)
 
